theories/Bilinear.v
@@ -1,0 +1,148 @@
+Require Import Grisette.Eval.
+Require Import Grisette.Terminate.
+Require Import Grisette.GeneralTactics.
+Require Import Grisette.Union.
+Require Import Grisette.SymBoolOp.
+Require Import Grisette.MergingStrategy.
+Require Import Grisette.SubStrategy.
+Require Import Grisette.Deterministic.
+Require Import Grisette.Invariant.
+Require Import Lia.
+Require Import Program.
+Require Import Coq.ZArith.BinInt.
+Require Import Coq.Arith.PeanoNat.
+Open Scope Z.
+Open Scope nat.
+
+Definition max_step {T} (t : EvalTerms T) : nat :=
+  match t with
+  | EvalValue _ _ => 0
+  | MrgIf ms c t f => 4 + 4 * ms_depth ms * (union_size t + union_size f)
+  | SSMrgIf ms c t f => 1 + 4 * ms_depth ms * (union_size t + union_size f)
+  | ISMrgIf ms c t f => 2 + 4 * ms_depth ms * (union_size t + union_size f)
+  | SIMrgIf ms c t f => 2 + 4 * ms_depth ms * (union_size t + union_size f)
+  | IIMrgIf ms c t f => 3 + 4 * ms_depth ms * (union_size t + union_size f)
+  end.
+
+Theorem linear': forall {T n t} {ms : MergingStrategy T n} {step1},
+  EvalTermsGood ms t ->
+  forall {u1},
+  t ==>(step1) (EvalValue ms u1) ->
+  step1 <= max_step t.
+Proof.
+  intros.
+  assert (good:exists n1 (ms1 : MergingStrategy T n1), EvalTermsGood ms1 t).
+  { exists n, ms. assumption. }
+  generalize dependent n.
+  generalize dependent u1.
+  generalize dependent step1.
+  apply EvalTerms_ind' with (t := t); intros; subst; eauto.
+  all: inversion_initial_eval_good; simpl in *; try solve [exfalso; eauto].
+  { invcd H1; try lia. }
+  { destruct b;
+    invcd H3; simpl in *; try solve [exfalso; auto];
+    lia.
+  }
+  { invcd H4; simpl in *; try solve [exfalso; auto]. 
+    lia.
+  }
+  1-4: invcd H3; simpl in *; try solve [exfalso; auto];
+    destruct ms; simpl in *; try solve [exfalso; auto].
+  { rewrite Nat.add_1_r; apply le_n_S; apply le_S; apply le_S; rewrite <- (Nat.add_0_r d).
+    eapply H1; eauto with eval;
+      invcd H2; econstructor; eauto with union. }
+  { rewrite Nat.add_1_r; apply le_n_S; apply le_S; rewrite <- (Nat.add_0_r d).
+    eapply H1; eauto with eval;
+      invcd H2; econstructor; eauto with union. }
+  { rewrite Nat.add_1_r; apply le_n_S; apply le_S; rewrite <- (Nat.add_0_r d).
+    eapply H1; eauto with eval;
+      invcd H2; econstructor; eauto with union. }
+  { rewrite Nat.add_1_r; apply le_n_S; rewrite <- (Nat.add_0_r d).
+    eapply H1; eauto with eval;
+      invcd H2; econstructor; eauto with union. }
+
+  Ltac preprocess :=
+    match goal with
+    | [ H1 : EvalTermsGood ?ms ?t,
+        H2 : ?t ==>(_) EvalValue ?ms ?u1 |- _ ] =>
+      invcd H1; invcd H2; try solve_aiu;
+      repeat aiu_simplify; repeat find_same
+    end.
+  Ltac unz_aux v :=
+    match v with
+    | S ?v' => unz_aux v' 
+    | ?v1 + ?v2 => unz_aux v1; unz_aux v2
+    | ?v1 * ?v2 => unz_aux v1; unz_aux v2
+    | union_size ?u => assert (union_size u > 0) by eauto with union
+    | ms_depth (SortedStrategy ?n _ _) => assert (n > 0) by eauto with inv
+    | _ => auto
+    end.
+
+  Ltac unz :=
+    match goal with
+    | [ |- _ <= ?t ] => unz_aux t
+    end.
+  all: preprocess; unz; unfold ms_depth in *; simpl in *; auto 1.
+
+  Ltac try1 :=
+    match goal with
+    | [ H : forall step1 u1 n ms, (EvalTermsGood ms (?op ?ms1 ?c ?t0 ?ff)) -> ?H2 -> step1 <= _,
+        H2 : ?op ?ms1 ?c ?t0 ?ff ==>(?step) EvalValue ?ms1 ?u |- _] =>
+      let He := fresh "H" in
+      assert (He:EvalTermsGood ms1 (op ms1 c t0 ff)) by (econstructor; eauto with inv union);
+      specialize (H step u _ ms1 He); intuition; nia
+    end.
+  all: try solve [try1].
+
+  { assert (EvalTermsGood s0 (MrgIf s0 c t0 f)).
+    { assert (ProperStrategy P (SortedStrategy n ind sub0)) by eauto 2 with inv.
+      specialize (all_in_union_left_most' H0); simpl; intros.
+      specialize (proper_ms_sub_from_subfunc H12 H13 H2) as [Psub ?].
+      assert (HieraricalMergingInv Psub s0 t0) by eauto 2 with subinv.
+      assert (HieraricalMergingInv Psub s0 f) by eauto 2 with subinv.
+      econstructor; eauto.
+    }
+    specialize (H3 _ _ _ _ H12 H24).
+    nia.
+  }
+
+  { assert (EvalTermsGood s0 (MrgIf s0 c t0 ft)).
+    { assert (ProperStrategy P (SortedStrategy n ind sub0)) by eauto 2 with inv.
+      specialize (all_in_union_left_most' H0); simpl; intros.
+      specialize (proper_ms_sub_from_subfunc H15 H20 H4) as [Psub ?].
+      assert (HieraricalMergingInv Psub s0 t0) by eauto 2 with subinv.
+      assert (HieraricalMergingInv Psub s0 ft) by eauto 3 with subinv inv.
+      econstructor; eauto.
+    }
+    specialize (H5 _ _ _ _ H15 H30).
+    nia.
+  }
+
+  { assert (EvalTermsGood s0 (MrgIf s0 c tt f)).
+    { assert (ProperStrategy P (SortedStrategy n ind sub0)) by eauto 2 with inv.
+      specialize (all_in_union_left_most' H0); simpl; intros.
+      specialize (proper_ms_sub_from_subfunc H15 H20 H4) as [Psub ?].
+      assert (HieraricalMergingInv Psub s0 tt) by eauto 3 with subinv inv.
+      assert (HieraricalMergingInv Psub s0 f) by eauto 2 with subinv.
+      econstructor; eauto.
+    }
+    specialize (H5 _ _ _ _ H15 H30).
+    unfold ms_depth in *; simpl in *.
+    nia.
+  }
+
+  { assert (EvalTermsGood (SortedStrategy n ind sub0) (MrgIf (SortedStrategy n ind sub0) c tf ff))
+      by (econstructor; eauto 2 with inv).
+    specialize (H8 _ _ _ _ H23 H38).
+    assert (EvalTermsGood s0 (MrgIf s0 c tt ft)).
+    { assert (ProperStrategy P (SortedStrategy n ind sub0)) by eauto 2 with inv.
+      specialize (all_in_union_left_most' H0); simpl; intros.
+      specialize (proper_ms_sub_from_subfunc H24 H25 H6) as [Psub ?].
+      assert (HieraricalMergingInv Psub s0 tt) by eauto 3 with subinv inv.
+      assert (HieraricalMergingInv Psub s0 ft) by eauto 3 with subinv inv.
+      econstructor; eauto.
+    }
+    specialize (H7 _ _ _ _ H24 H37).
+    nia.
+  }
+Qed.  
