theories/Deterministic.v
@@ -6,14 +6,15 @@ Require Import Grisette.GeneralTactics.
 Require Import Grisette.MergingStrategy.
 Require Import Grisette.SubStrategy.
 Require Import Lia.
+Require Import Coq.Arith.PeanoNat.
 
 Ltac remove_star :=
   match goal with
-  | [ H: MrgIf _ _ _ _ ==>* EvalValue _ _ |- _] => apply eval_star_mrgif in H
-  | [ H: SSMrgIf _ _ _ _ ==>* EvalValue _ _ |- _ ] => apply eval_star_ss in H
-  | [ H: ISMrgIf _ _ _ _ ==>* EvalValue _ _ |- _ ] => apply eval_star_is in H
-  | [ H: SIMrgIf _ _ _ _ ==>* EvalValue _ _ |- _ ] => apply eval_star_si in H
-  | [ H: IIMrgIf _ _ _ _ ==>* EvalValue _ _ |- _ ] => apply eval_star_ii in H
+  | [ H: MrgIf _ _ _ _ ==>(_)* EvalValue _ _ |- _] => apply eval_star_mrgif in H
+  | [ H: SSMrgIf _ _ _ _ ==>(_)* EvalValue _ _ |- _ ] => apply eval_star_ss in H
+  | [ H: ISMrgIf _ _ _ _ ==>(_)* EvalValue _ _ |- _ ] => apply eval_star_is in H
+  | [ H: SIMrgIf _ _ _ _ ==>(_)* EvalValue _ _ |- _ ] => apply eval_star_si in H
+  | [ H: IIMrgIf _ _ _ _ ==>(_)* EvalValue _ _ |- _ ] => apply eval_star_ii in H
   end.
 
 Ltac find_same :=
@@ -23,12 +24,39 @@ Ltac find_same :=
     | [ H1 : _ = ?x, H2 : _ = ?x |- _ ] => rewrite <- H1 in H2; invcd H2
   end.
 
-Theorem determinstic': forall {T n t} {ms : MergingStrategy T n},
+Lemma union_sub_rewrite_t :
+  forall {T} c (t1 t2 f : Union T), If c t1 f = If c t2 f <-> t1 = t2.
+Proof.
+  intros.
+  split; intros.
+  invcd H; auto.
+  subst. auto.
+Qed.
+
+Lemma union_sub_rewrite_f :
+  forall {T} c (t f1 f2 : Union T), If c t f1 = If c t f2 <-> f1 = f2.
+Proof.
+  intros.
+  split; intros.
+  invcd H; auto.
+  subst. auto.
+Qed.
+
+Lemma union_sub_rewrite_tf :
+  forall {T} c (t1 t2 f1 f2 : Union T), If c t1 f1 = If c t2 f2 <-> t1 = t2 /\ f1 = f2.
+Proof.
+  intros.
+  split; intros.
+  invcd H; auto.
+  intuition; subst; auto.
+Qed.
+
+Theorem determinstic': forall {T n t} {ms : MergingStrategy T n} {step1 step2},
   EvalTermsGood ms t ->
   forall {u1 u2},
-  t ==>* (EvalValue ms u1) ->
-  t ==>* (EvalValue ms u2) ->
-  u1 = u2.
+  t ==>(step1)* (EvalValue ms u1) ->
+  t ==>(step2)* (EvalValue ms u2) ->
+  u1 = u2 /\ step1 = step2.
 Proof.
   intros.
   assert (good:exists n1 (ms1 : MergingStrategy T n1), EvalTermsGood ms1 t).
@@ -36,14 +64,17 @@ Proof.
   generalize dependent n.
   generalize dependent u1.
   generalize dependent u2.
+  generalize dependent step1.
+  generalize dependent step2.
   apply EvalTerms_ind' with (t := t); intros; subst; eauto.
   all: inversion_initial_eval_good; simpl in *; try solve [exfalso; eauto].
   all: repeat remove_star.
   { specialize (value_evaluate_to_value H1).
     specialize (value_evaluate_to_value H2).
     intros.
+    intuition; try lia.
+    invcd H6.
     invcd H3.
-    invcd H4.
     auto.
   }
   { destruct b;
@@ -53,36 +84,38 @@ Proof.
   }
   { invcd H4; simpl in *; try solve [exfalso; auto]. 
     invcd H5; simpl in *; try solve [exfalso; auto]. 
-    rewrite H8 in H7. invcd H7. auto.
+    rewrite H12 in H14. invcd H14. auto.
   }
   1-4: invcd H3; simpl in *; try solve [exfalso; auto];
-    invcd H4; simpl in *; try solve [exfalso; auto]; 
+    invcd H4; simpl in *; try solve [exfalso; auto];
     destruct ms; simpl in *; try solve [exfalso; auto];
-    eapply H1; eauto with eval;
-    invcd H2;
-    econstructor; eauto with union.
-
+    assert (Hd:d + 1 = d0 + 1 <-> d + 0 = d0 + 0) by lia; rewrite Hd;
+    eapply H1; eauto with eval; invcd H2; econstructor; eauto with union.
   Ltac preprocess :=
     match goal with
     | [ H1 : EvalTermsGood ?ms ?t,
-        H2 : ?t ==>* EvalValue ?ms ?u1,
-        H3 : ?t ==>* EvalValue ?ms ?u2 |- _ ] =>
+        H2 : ?t ==>(_)* EvalValue ?ms ?u1,
+        H3 : ?t ==>(_)* EvalValue ?ms ?u2 |- _ ] =>
       invcd H1; repeat remove_star; invcd H2; try solve_aiu; invcd H3; try solve_aiu;
       repeat aiu_simplify; repeat find_same
     end.
   all: preprocess; auto 1.
-  (* SSLt (auto) *)
 
   Ltac try1 :=
     match goal with
-    | [ H : forall u2 u1 n ms, _ -> _ ==>* _ -> _ ==>* _ -> u1 = u2 |- _] =>
+    | [ H : forall step2 step1 u2 u1 n ms, _ -> _ ==>(step1)* _ -> _ ==>(step2)* _ -> u1 = u2 /\ step1 = step2 |- _] =>
       eapply H
     end.
 
-  all: try solve [try f_equal; try1; eauto 2 with eval; econstructor; eauto 2 with union inv].
+  all: try solve [intuition; try lia; try f_equal; eauto].
+  all: try solve [
+    assert (Hd:d0 + 1 = d + 1 <-> d0 + 0 = d + 0) by lia; rewrite Hd;
+    try rewrite union_sub_rewrite_t; try rewrite union_sub_rewrite_f;
+    try1; eauto 2 with eval; econstructor; eauto 2 with union inv].
 
   (* SSEq *)
-  { eapply H3; eauto with eval.
+  { assert (Hd:d0 + 1 = d + 1 <-> d0 + 0 = d + 0) by lia; rewrite Hd;
+    eapply H3; eauto with eval.
     assert (ProperStrategy P0 (SortedStrategy n ind sub0)) by eauto 2 with inv.
     specialize (all_in_union_left_most' H0); simpl; intros.
     specialize (proper_ms_sub_from_subfunc H4 H5 H2) as [Psub ?].
@@ -92,7 +125,8 @@ Proof.
   }
 
   (* SIEq *)
-  { f_equal.
+  { assert (Hd:d0 + 1 = d + 1 <-> d0 + 0 = d + 0) by lia; rewrite Hd;
+    rewrite union_sub_rewrite_t.
     eapply H5; eauto with eval.
     assert (ProperStrategy P0 (SortedStrategy n ind sub0)) by eauto 2 with inv.
     specialize (all_in_union_left_most' H0); simpl; intros.
@@ -103,7 +137,8 @@ Proof.
   }
 
   (* ISEq *)
-  { f_equal.
+  { assert (Hd:d0 + 1 = d + 1 <-> d0 + 0 = d + 0) by lia; rewrite Hd;
+    rewrite union_sub_rewrite_t.
     eapply H5; eauto 2 with eval.
     assert (ProperStrategy P0 (SortedStrategy n ind sub0)) by eauto 2 with inv.
     specialize (all_in_union_left_most' H0); simpl; intros.
@@ -114,16 +149,21 @@ Proof.
   }
 
   (* IIEq *)
-  { f_equal.
-    - eapply H7; eauto 2 with eval.
-      assert (ProperStrategy P0 (SortedStrategy n ind sub0)) by eauto 2 with inv.
-      specialize (all_in_union_left_most' H0); simpl; intros.
-      specialize (proper_ms_sub_from_subfunc H9 H10 H6) as [Psub ?].
-      assert (HieraricalMergingInv Psub s1 tt) by eauto 3 with subinv inv.
-      assert (HieraricalMergingInv Psub s1 ft) by eauto 3 with subinv inv.
-      econstructor; eauto.
-    - eapply H8; eauto 2 with eval.
-      econstructor; eauto with inv.
-   }
+  { assert ((t'0 = t' /\ d0 + 0 = d1 + 0) /\ (f'0 = f' /\ d3 + 0 = d2 + 0)).
+    { split.
+      - eapply H7; eauto 2 with eval.
+        assert (ProperStrategy P0 (SortedStrategy n ind sub0)) by eauto 2 with inv.
+        specialize (all_in_union_left_most' H0); simpl; intros.
+        specialize (proper_ms_sub_from_subfunc H9 H10 H6) as [Psub ?].
+        assert (HieraricalMergingInv Psub s1 tt) by eauto 3 with subinv inv.
+        assert (HieraricalMergingInv Psub s1 ft) by eauto 3 with subinv inv.
+        econstructor; eauto.
+      - eapply H8; eauto 2 with eval.
+        econstructor; eauto with inv.
+    }
+    intuition.
+    - f_equal; auto.
+    - lia.
+  }
 Qed.
 
