theories/Eval.v
@@ -143,63 +143,63 @@ Qed.
 #[global] Hint Resolve good_implies_proper_strategy : eval.
 
 
-Inductive EvalRule {T} : EvalTerms T -> EvalTerms T -> Prop :=
+Inductive EvalRule {T} : EvalTerms T -> EvalTerms T -> nat -> Prop :=
   | MrgIfTrue : forall {n} (ms : MergingStrategy T n) t f,
-    EvalRule (MrgIf ms (ConSymBool true) t f) (EvalValue ms t)
+    EvalRule (MrgIf ms (ConSymBool true) t f) (EvalValue ms t) 1
   | MrgIfFalse : forall {n} (ms : MergingStrategy T n) t f,
-    EvalRule (MrgIf ms (ConSymBool false) t f) (EvalValue ms f)
+    EvalRule (MrgIf ms (ConSymBool false) t f) (EvalValue ms f) 1
   | MrgIfSimple : forall m c t f r,
     m c t f = Some r ->
     ~ IsConc c ->
-    EvalRule (MrgIf (SimpleStrategy m) c (Single t) (Single f)) (EvalValue (SimpleStrategy m) (Single r))
-  | MrgIfSortedSS : forall {n} (s : MergingStrategy T n) c t f r,
+    EvalRule (MrgIf (SimpleStrategy m) c (Single t) (Single f)) (EvalValue (SimpleStrategy m) (Single r)) 1
+  | MrgIfSortedSS : forall {n} (s : MergingStrategy T n) c t f r {d},
     is_sorted_strategy s ->
     ~ IsConc c ->
     is_single t ->
     is_single f ->
-    EvalRule (SSMrgIf s c t f) (EvalValue s r) ->
-    EvalRule (MrgIf s c t f) (EvalValue s r)
-  | MrgIfSortedSI : forall {n} (s : MergingStrategy T n) c t f r,
+    EvalRule (SSMrgIf s c t f) (EvalValue s r) d ->
+    EvalRule (MrgIf s c t f) (EvalValue s r) (d + 1)
+  | MrgIfSortedSI : forall {n} (s : MergingStrategy T n) c t f r {d},
     is_sorted_strategy s ->
     ~ IsConc c ->
     is_single t ->
     is_if f ->
-    EvalRule (SIMrgIf s c t f) (EvalValue s r) ->
-    EvalRule (MrgIf s c t f) (EvalValue s r)
-  | MrgIfSortedIS : forall {n} (s : MergingStrategy T n) c t f r,
+    EvalRule (SIMrgIf s c t f) (EvalValue s r) d ->
+    EvalRule (MrgIf s c t f) (EvalValue s r) (d + 1)
+  | MrgIfSortedIS : forall {n} (s : MergingStrategy T n) c t f r {d},
     is_sorted_strategy s ->
     ~ IsConc c ->
     is_if t ->
     is_single f ->
-    EvalRule (ISMrgIf s c t f) (EvalValue s r) ->
-    EvalRule (MrgIf s c t f) (EvalValue s r)
-  | MrgIfSortedII : forall {n} (s : MergingStrategy T n) c t f r,
+    EvalRule (ISMrgIf s c t f) (EvalValue s r) d ->
+    EvalRule (MrgIf s c t f) (EvalValue s r) (d + 1)
+  | MrgIfSortedII : forall {n} (s : MergingStrategy T n) c t f r {d},
     is_sorted_strategy s ->
     ~ IsConc c ->
     is_if t ->
     is_if f ->
-    EvalRule (IIMrgIf s c t f) (EvalValue s r) ->
-    EvalRule (MrgIf s c t f) (EvalValue s r)
+    EvalRule (IIMrgIf s c t f) (EvalValue s r) d ->
+    EvalRule (MrgIf s c t f) (EvalValue s r) (d + 1)
   | SSLt : forall {n} ind sub c t f ti fi,
     AllInUnion (fun x => ind x = Some ti) t ->
     AllInUnion (fun x => ind x = Some fi) f ->
     (ti < fi)%Z ->
-    EvalRule (SSMrgIf (SortedStrategy n ind sub) c t f) (EvalValue (SortedStrategy n ind sub) (If c t f))
-  | SSEq : forall {n} ind sub c t f i n1 s (ev : n1 < n) r,
+    EvalRule (SSMrgIf (SortedStrategy n ind sub) c t f) (EvalValue (SortedStrategy n ind sub) (If c t f)) 1
+  | SSEq : forall {n} ind sub c t f i n1 s (ev : n1 < n) r {d},
     AllInUnion (fun x => ind x = Some i) t ->
     AllInUnion (fun x => ind x = Some i) f ->
     sub i = Some (MSSubLt s ev) ->
-    EvalRule (MrgIf s c t f) (EvalValue s r) ->
-    EvalRule (SSMrgIf (SortedStrategy n ind sub) c t f) (EvalValue (SortedStrategy n ind sub) r)
+    EvalRule (MrgIf s c t f) (EvalValue s r) d ->
+    EvalRule (SSMrgIf (SortedStrategy n ind sub) c t f) (EvalValue (SortedStrategy n ind sub) r) (d + 1)
   | SSGt : forall {n} ind sub c t f ti fi,
     AllInUnion (fun x => ind x = Some ti) t ->
     AllInUnion (fun x => ind x = Some fi) f ->
     (ti > fi)%Z ->
-    EvalRule (SSMrgIf (SortedStrategy n ind sub) c t f) (EvalValue (SortedStrategy n ind sub) (If (pnegsb c) f t))
-  | SIDeg : forall {n} ind sub c t f fi r,
+    EvalRule (SSMrgIf (SortedStrategy n ind sub) c t f) (EvalValue (SortedStrategy n ind sub) (If (pnegsb c) f t)) 1
+  | SIDeg : forall {n} ind sub c t f fi r {d},
     AllInUnion (fun x => ind x = Some fi) f ->
-    EvalRule (SSMrgIf (SortedStrategy n ind sub) c t f) (EvalValue (SortedStrategy n ind sub) r) ->
-    EvalRule (SIMrgIf (SortedStrategy n ind sub) c t f) (EvalValue (SortedStrategy n ind sub) r)
+    EvalRule (SSMrgIf (SortedStrategy n ind sub) c t f) (EvalValue (SortedStrategy n ind sub) r) d ->
+    EvalRule (SIMrgIf (SortedStrategy n ind sub) c t f) (EvalValue (SortedStrategy n ind sub) r) (d + 1)
   | SILt : forall {n} ind sub c t fc ft ff ti fti ffi,
     AllInUnion (fun x => ind x = Some ti) t ->
     AllInUnion (fun x => ind x = Some fti) ft ->
@@ -207,47 +207,47 @@ Inductive EvalRule {T} : EvalTerms T -> EvalTerms T -> Prop :=
     (fti <> ffi)%Z ->
     (ti < fti)%Z ->
     EvalRule (SIMrgIf (SortedStrategy n ind sub) c t (If fc ft ff))
-             (EvalValue (SortedStrategy n ind sub) (If c t (If fc ft ff)))
-  | SIEq : forall {n} ind sub c t fc ft ff ti ffi n1 s t' (ev : n1 < n),
+             (EvalValue (SortedStrategy n ind sub) (If c t (If fc ft ff))) 1
+  | SIEq : forall {n} ind sub c t fc ft ff ti ffi n1 s t' (ev : n1 < n) {d},
     AllInUnion (fun x => ind x = Some ti) t ->
     AllInUnion (fun x => ind x = Some ti) ft ->
     ind (left_most ff) = Some ffi ->
     (ti <> ffi)%Z ->
     sub ti = Some (MSSubLt s ev) ->
-    EvalRule (MrgIf s c t ft) (EvalValue s t') ->
+    EvalRule (MrgIf s c t ft) (EvalValue s t') d ->
     EvalRule (SIMrgIf (SortedStrategy n ind sub) c t (If fc ft ff))
-             (EvalValue (SortedStrategy n ind sub) (If (porsb c fc) t' ff))
-  | SIGt : forall {n} ind sub c t fc ft ff ti fti ffi f',
+             (EvalValue (SortedStrategy n ind sub) (If (porsb c fc) t' ff)) (d + 1)
+  | SIGt : forall {n} ind sub c t fc ft ff ti fti ffi f' {d},
     AllInUnion (fun x => ind x = Some ti) t ->
     AllInUnion (fun x => ind x = Some fti) ft ->
     ind (left_most ff) = Some ffi ->
     (fti <> ffi)%Z ->
     (ti > fti)%Z ->
-    EvalRule (MrgIf (SortedStrategy n ind sub) c t ff) (EvalValue (SortedStrategy n ind sub) f') ->
+    EvalRule (MrgIf (SortedStrategy n ind sub) c t ff) (EvalValue (SortedStrategy n ind sub) f') d ->
     EvalRule (SIMrgIf (SortedStrategy n ind sub) c t (If fc ft ff))
-             (EvalValue (SortedStrategy n ind sub) (If (pandsb (pnegsb c) fc) ft f'))
-  | ISDeg : forall {n} ind sub c t f ti r,
+             (EvalValue (SortedStrategy n ind sub) (If (pandsb (pnegsb c) fc) ft f')) (d + 1)
+  | ISDeg : forall {n} ind sub c t f ti r {d},
     AllInUnion (fun x => ind x = Some ti) t ->
-    EvalRule (SSMrgIf (SortedStrategy n ind sub) c t f) (EvalValue (SortedStrategy n ind sub) r) ->
-    EvalRule (ISMrgIf (SortedStrategy n ind sub) c t f) (EvalValue (SortedStrategy n ind sub) r)
-  | ISLt : forall {n} ind sub c tc tt tf f tti tfi fi f',
+    EvalRule (SSMrgIf (SortedStrategy n ind sub) c t f) (EvalValue (SortedStrategy n ind sub) r) d ->
+    EvalRule (ISMrgIf (SortedStrategy n ind sub) c t f) (EvalValue (SortedStrategy n ind sub) r) (d + 1)
+  | ISLt : forall {n} ind sub c tc tt tf f tti tfi fi f' {d},
     AllInUnion (fun x => ind x = Some tti) tt ->
     AllInUnion (fun x => ind x = Some fi) f ->
     ind (left_most tf) = Some tfi ->
     (tti <> tfi)%Z ->
     (tti < fi)%Z ->
-    EvalRule (MrgIf (SortedStrategy n ind sub) c tf f) (EvalValue (SortedStrategy n ind sub) f') ->
+    EvalRule (MrgIf (SortedStrategy n ind sub) c tf f) (EvalValue (SortedStrategy n ind sub) f') d ->
     EvalRule (ISMrgIf (SortedStrategy n ind sub) c (If tc tt tf) f)
-             (EvalValue (SortedStrategy n ind sub) (If (pandsb c tc) tt f'))
-  | ISEq : forall {n} ind sub c tc tt tf f tfi fi n1 s t' (ev : n1 < n),
+             (EvalValue (SortedStrategy n ind sub) (If (pandsb c tc) tt f')) (d + 1)
+  | ISEq : forall {n} ind sub c tc tt tf f tfi fi n1 s t' (ev : n1 < n) {d},
     AllInUnion (fun x => ind x = Some fi) tt ->
     AllInUnion (fun x => ind x = Some fi) f ->
     ind (left_most tf) = Some tfi ->
     (tfi <> fi)%Z ->
     sub fi = Some (MSSubLt s ev) ->
-    EvalRule (MrgIf s c tt f) (EvalValue s t') ->
+    EvalRule (MrgIf s c tt f) (EvalValue s t') d ->
     EvalRule (ISMrgIf (SortedStrategy n ind sub) c (If tc tt tf) f)
-             (EvalValue (SortedStrategy n ind sub) (If (porsb (pnegsb c) tc) t' tf))
+             (EvalValue (SortedStrategy n ind sub) (If (porsb (pnegsb c) tc) t' tf)) (d + 1)
   | ISGt : forall {n} ind sub c tc tt tf f tti tfi fi,
     AllInUnion (fun x => ind x = Some tti) tt ->
     AllInUnion (fun x => ind x = Some fi) f ->
@@ -255,23 +255,23 @@ Inductive EvalRule {T} : EvalTerms T -> EvalTerms T -> Prop :=
     (tti <> tfi)%Z ->
     (tti > fi)%Z ->
     EvalRule (ISMrgIf (SortedStrategy n ind sub) c (If tc tt tf) f)
-             (EvalValue (SortedStrategy n ind sub) (If (pnegsb c) f (If tc tt tf)))
-  | IIDeg1 : forall {n} ind sub c t f ti r,
+             (EvalValue (SortedStrategy n ind sub) (If (pnegsb c) f (If tc tt tf))) 1
+  | IIDeg1 : forall {n} ind sub c t f ti r {d},
     AllInUnion (fun x => ind x = Some ti) t ->
     EvalRule (SIMrgIf (SortedStrategy n ind sub) c t f)
-                                  (EvalValue (SortedStrategy n ind sub) r) ->
+                                  (EvalValue (SortedStrategy n ind sub) r) d ->
     EvalRule (IIMrgIf (SortedStrategy n ind sub) c t f)
-             (EvalValue (SortedStrategy n ind sub) r)
-  | IIDeg2 : forall {n} ind sub c tc tt tf f tti tfi fi r,
+             (EvalValue (SortedStrategy n ind sub) r) (d + 1)
+  | IIDeg2 : forall {n} ind sub c tc tt tf f tti tfi fi r {d},
     AllInUnion (fun x => ind x = Some tti) tt ->
     AllInUnion (fun x => ind x = Some fi) f ->
     ind (left_most tf) = Some tfi ->
     (tti <> tfi)%Z ->
     EvalRule (ISMrgIf (SortedStrategy n ind sub) c (If tc tt tf) f)
-                                  (EvalValue (SortedStrategy n ind sub) r) ->
+                                  (EvalValue (SortedStrategy n ind sub) r) d ->
     EvalRule (IIMrgIf (SortedStrategy n ind sub) c (If tc tt tf) f)
-             (EvalValue (SortedStrategy n ind sub) r)
-  | IILt : forall {n} ind sub c tc tt tf fc ft ff tti tfi fti ffi f',
+             (EvalValue (SortedStrategy n ind sub) r) (d + 1)
+  | IILt : forall {n} ind sub c tc tt tf fc ft ff tti tfi fti ffi f' {d},
     AllInUnion (fun x => ind x = Some tti) tt ->
     ind (left_most tf) = Some tfi ->
     AllInUnion (fun x => ind x = Some fti) ft ->
@@ -280,10 +280,10 @@ Inductive EvalRule {T} : EvalTerms T -> EvalTerms T -> Prop :=
     (fti <> ffi)%Z ->
     (tti < fti)%Z ->
     EvalRule (MrgIf (SortedStrategy n ind sub) c tf (If fc ft ff))
-                                  (EvalValue (SortedStrategy n ind sub) f') ->
+                                  (EvalValue (SortedStrategy n ind sub) f') d ->
     EvalRule (IIMrgIf (SortedStrategy n ind sub) c (If tc tt tf) (If fc ft ff))
-             (EvalValue (SortedStrategy n ind sub) (If (pandsb c tc) tt f'))
-  | IIEq : forall {n} ind sub c tc tt tf fc ft ff tfi fti ffi n1 s (ev : n1 < n) t' f',
+             (EvalValue (SortedStrategy n ind sub) (If (pandsb c tc) tt f')) (d + 1)
+  | IIEq : forall {n} ind sub c tc tt tf fc ft ff tfi fti ffi n1 s (ev : n1 < n) t' f' {d1 d2},
     AllInUnion (fun x => ind x = Some fti) tt -> 
     ind (left_most tf) = Some tfi ->
     AllInUnion (fun x => ind x = Some fti) ft ->
@@ -291,12 +291,12 @@ Inductive EvalRule {T} : EvalTerms T -> EvalTerms T -> Prop :=
     (fti <> tfi)%Z ->
     (fti <> ffi)%Z ->
     sub fti = Some (MSSubLt s ev) ->
-    EvalRule (MrgIf s c tt ft) (EvalValue s t') ->
+    EvalRule (MrgIf s c tt ft) (EvalValue s t') d1 ->
     EvalRule (MrgIf (SortedStrategy n ind sub) c tf ff)
-                                  (EvalValue (SortedStrategy n ind sub) f') ->
+                                  (EvalValue (SortedStrategy n ind sub) f') d2 ->
     EvalRule (IIMrgIf (SortedStrategy n ind sub) c (If tc tt tf) (If fc ft ff))
-             (EvalValue (SortedStrategy n ind sub) (If (pitesb c tc fc) t' f'))
-  | IIGt : forall {n} ind sub c tc tt tf fc ft ff tti tfi fti ffi f',
+             (EvalValue (SortedStrategy n ind sub) (If (pitesb c tc fc) t' f')) (d1 + d2 + 1)
+  | IIGt : forall {n} ind sub c tc tt tf fc ft ff tti tfi fti ffi f' {d},
     AllInUnion (fun x => ind x = Some tti) tt ->
     ind (left_most tf) = Some tfi ->
     AllInUnion (fun x => ind x = Some fti) ft ->
@@ -305,13 +305,13 @@ Inductive EvalRule {T} : EvalTerms T -> EvalTerms T -> Prop :=
     (fti <> ffi)%Z ->
     (tti > fti)%Z ->
     EvalRule (MrgIf (SortedStrategy n ind sub) c (If tc tt tf) ff)
-                                  (EvalValue (SortedStrategy n ind sub) f') ->
+                                  (EvalValue (SortedStrategy n ind sub) f') d ->
     EvalRule (IIMrgIf (SortedStrategy n ind sub) c (If tc tt tf) (If fc ft ff))
-             (EvalValue (SortedStrategy n ind sub) (If (pandsb (pnegsb c) fc) ft f')).
+             (EvalValue (SortedStrategy n ind sub) (If (pandsb (pnegsb c) fc) ft f')) (d + 1).
 
 #[global] Hint Constructors EvalRule : eval.
 
-Notation "t1 '==>' t2" := (EvalRule t1 t2) (at level 75).
+Notation "t1 '==>(' n ')' t2" := (EvalRule t1 t2 n) (at level 75).
 
 Definition metric {T} (t : EvalTerms T) : nat :=
   match t with
@@ -1055,14 +1055,17 @@ Proof.
   rewrite H0 in H2. invcd H2. solve_aiu.
 Qed.
 
-Arguments clos_refl_trans_1n {A}.
-#[global] Hint Constructors clos_refl_trans_1n : eval.
+Inductive MultiStepEvalRule {T} (x : EvalTerms T): EvalTerms T -> nat -> Prop :=
+  | EvalOne : MultiStepEvalRule x x 0
+  | EvalTrans : forall {y z : EvalTerms T} {nxy nyz}, x ==>(nxy)y -> MultiStepEvalRule y z nyz -> MultiStepEvalRule x z (nxy + nyz).
 
-Notation "t1 '==>*' t2" := (clos_refl_trans_1n EvalRule t1 t2) (at level 75).
+#[global] Hint Constructors MultiStepEvalRule : eval.
+
+Notation "t1 '==>(' n ')*' t2" := (MultiStepEvalRule t1 t2 n) (at level 75).
 
 Lemma value_evaluate_to_value : forall {T n1} {ms1 : MergingStrategy T n1}
-  {u1} {t2},
-  EvalValue ms1 u1 ==>* t2 -> EvalValue ms1 u1 = t2.
+  {u1} {t2} {step},
+  EvalValue ms1 u1 ==>(step)* t2 -> EvalValue ms1 u1 = t2 /\ step = 0.
 Proof.
   intros.
   invcd H; auto.
@@ -1071,78 +1074,81 @@ Qed.
 
 Ltac invcd_eval_value :=
   match goal with
-  | [ H: EvalValue ?ms1 ?r1 ==>* ?t |- _] =>
-    apply value_evaluate_to_value in H; invcd H
+  | [ H: EvalValue ?ms1 ?r1 ==>(?step)* ?t |- _] =>
+    let H1 := fresh "H" in
+    apply value_evaluate_to_value in H as [H H1]; invcd H
   end.
 
 #[global] Hint Resolve value_evaluate_to_value : eval.
 
-Lemma eval_star_is_eq_or_onestep : forall {T} {t1 t2 : EvalTerms T},
-  t1 ==>* t2 -> t1 = t2 \/ t1 ==> t2.
+Lemma eval_star_is_eq_or_onestep : forall {T} {t1 t2 : EvalTerms T} {step},
+  t1 ==>(step)* t2 -> (t1 = t2 /\ step = 0) \/ t1 ==>(step) t2.
 Proof.
   intros.
   invcd H; eauto.
-  invcd H0; try invcd_eval_value; right; eauto with eval.
+  invcd H0; try invcd_eval_value; right;
+  try rewrite <- plus_n_O;
+  eauto with eval. 
 Qed.
 
 #[global] Hint Resolve eval_star_is_eq_or_onestep : eval.
 
-Lemma eval_star_mrgif : forall {T n} {ms : MergingStrategy T n} c t f u,
-  MrgIf ms c t f ==>* EvalValue ms u ->
-  MrgIf ms c t f ==> EvalValue ms u.
+Lemma eval_star_mrgif : forall {T n} {ms : MergingStrategy T n} c t f u {step},
+  MrgIf ms c t f ==>(step)* EvalValue ms u ->
+  MrgIf ms c t f ==>(step) EvalValue ms u.
 Proof.
   intros.
   specialize (eval_star_is_eq_or_onestep H).
   intuition.
-  invcd H1.
+  invcd H0.
 Qed.
 
 #[global] Hint Resolve eval_star_mrgif : eval.
 
-Lemma eval_star_ss : forall {T n} {ms : MergingStrategy T n} c t f u,
-  SSMrgIf ms c t f ==>* EvalValue ms u ->
-  SSMrgIf ms c t f ==> EvalValue ms u.
+Lemma eval_star_ss : forall {T n} {ms : MergingStrategy T n} c t f u {step},
+  SSMrgIf ms c t f ==>(step)* EvalValue ms u ->
+  SSMrgIf ms c t f ==>(step) EvalValue ms u.
 Proof.
   intros.
   specialize (eval_star_is_eq_or_onestep H).
   intuition.
-  invcd H1.
+  invcd H0.
 Qed.
 
 #[global] Hint Resolve eval_star_ss : eval.
 
-Lemma eval_star_is : forall {T n} {ms : MergingStrategy T n} c t f u,
-  ISMrgIf ms c t f ==>* EvalValue ms u ->
-  ISMrgIf ms c t f ==> EvalValue ms u.
+Lemma eval_star_is : forall {T n} {ms : MergingStrategy T n} c t f u {step},
+  ISMrgIf ms c t f ==>(step)* EvalValue ms u ->
+  ISMrgIf ms c t f ==>(step) EvalValue ms u.
 Proof.
   intros.
   specialize (eval_star_is_eq_or_onestep H).
   intuition.
-  invcd H1.
+  invcd H0.
 Qed.
 
 #[global] Hint Resolve eval_star_is : eval.
 
-Lemma eval_star_si : forall {T n} {ms : MergingStrategy T n} c t f u,
-  SIMrgIf ms c t f ==>* EvalValue ms u ->
-  SIMrgIf ms c t f ==> EvalValue ms u.
+Lemma eval_star_si : forall {T n} {ms : MergingStrategy T n} c t f u {step},
+  SIMrgIf ms c t f ==>(step)* EvalValue ms u ->
+  SIMrgIf ms c t f ==>(step) EvalValue ms u.
 Proof.
   intros.
   specialize (eval_star_is_eq_or_onestep H).
   intuition.
-  invcd H1.
+  invcd H0.
 Qed.
 
 #[global] Hint Resolve eval_star_si : eval.
 
-Lemma eval_star_ii : forall {T n} {ms : MergingStrategy T n} c t f u,
-  IIMrgIf ms c t f ==>* EvalValue ms u ->
-  IIMrgIf ms c t f ==> EvalValue ms u.
+Lemma eval_star_ii : forall {T n} {ms : MergingStrategy T n} c t f u {step},
+  IIMrgIf ms c t f ==>(step)* EvalValue ms u ->
+  IIMrgIf ms c t f ==>(step) EvalValue ms u.
 Proof.
   intros.
   specialize (eval_star_is_eq_or_onestep H).
   intuition.
-  invcd H1.
+  invcd H0.
 Qed.
 
 #[global] Hint Resolve eval_star_ii : eval.
@@ -1154,7 +1160,7 @@ Theorem eval_do_not_change_index_subrt : forall {T n n1} {P ind sub} {i t} {Psub
   (if b
     then all_in_et (fun (x : T) => ind x = Some i) t
     else all_in_et (fun x => exists i1, ind x = Some i1 /\ (i1 > i)%Z) t) ->
-  forall u, t ==>* (EvalValue s u) ->
+  forall u step, t ==>(step)* (EvalValue s u) ->
   (if b
     then AllInUnion (fun (x : T) => ind x = Some i) u
     else AllInUnion (fun x => exists i1, ind x = Some i1 /\ (i1 > i)%Z) u).
@@ -1166,6 +1172,7 @@ Proof.
   generalize dependent sub.
   generalize dependent Psub.
   generalize dependent n1.
+  generalize dependent step.
   apply EvalTerms_ind' with (t := t); intros; try invcd_eval_value; subst; eauto.
   { invcd H6. destruct b; simpl in *; invcd_eval_rule H7;
     invcd_eval_value; intuition.
@@ -1174,21 +1181,21 @@ Proof.
     invcd H3.
     invcd H7. invcd_eval_rule H3.
     repeat invcd_eval_value.
-    rewrite H14 in H0. invcd H0.
+    rewrite H16 in H0. invcd H0.
     destruct b; simpl in *;
     invcd H6; invcd H0; invcd H3;
     eapply H1; clear H1; eauto; econstructor.
     1,3: clear H5 H4 sub H2 H Psub; eauto with inv.
     - invcd H5.
       eapply proper_ms_subt_simple_t.
-      3: apply H14.
+      3: apply H16.
       all: eauto.
     - destruct H7 as [i1 ?].
       invcd H5.
       exists i1.
       intuition.
       eapply proper_ms_subt_simple_t.
-      3: apply H14.
+      3: apply H16.
       all: eauto.
   }
   1-4: destruct b; simpl in *; destruct ms; simpl in H0; try solve [exfalso; auto];
@@ -1205,15 +1212,15 @@ Proof.
     all: invcd_eval_value.
     all: assert (i0 = i1) by eauto with union.
     all: subst.
-    all: rewrite H2 in H21; invcd H21.
-    all: clear H19 H20.
+    all: rewrite H2 in H22; invcd H22.
+    all: clear H20 H21.
     all: specialize (all_in_union_left_most' H0); simpl; intros.
     all: invcd H4.
     all: assert (ProperStrategy Psub (SortedStrategy n2 ind sub)) by eauto with sub.
     all: assert (ProperStrategy P0 (SortedStrategy n2 ind sub)) by eauto with inv.
     all: specialize (proper_ms_sub_from_subfunc H4 H7 H2) as [Psub' Hsub'].
     all: eapply H3; simpl in *.
-    5,10: econstructor; [apply H22|constructor].
+    5,10: econstructor; [apply H23|constructor].
     all: eauto.
     1,3: specialize (proper_ms_sub_from_subfunc H8 H7 H2) as [Psub'' Hsub''];
          econstructor; eapply hm_sub_hm; eauto.
@@ -1230,11 +1237,11 @@ Proof.
     all: invcd H6.
     all: invcd H5.
     1,5: invcd_eval_value;
-      eapply H1;[ | | | | econstructor; [apply H18|constructor]];
+      eapply H1;[ | | | | econstructor; [apply H19|constructor]];
       simpl; eauto with eval union.
     all: invcd H0;
       specialize (all_in_union_left_most' H12); simpl; intros;
-      rewrite H19 in H0; invcd H0;
+      rewrite H20 in H0; invcd H0;
       solve_aiu.
   }
   
@@ -1250,7 +1257,7 @@ Proof.
 
   (* SIEq *)
   1-2: assert (ti = ti0) by eauto with union; subst.
-  1-2: rewrite H4 in H28; invcd H28.
+  1-2: rewrite H4 in H29; invcd H29.
   1-2: constructor; eauto.
   1-2: assert (HieraricalMergingInv P0 (SortedStrategy n0 ind sub1) ft) by eauto with inv.
   1-2: assert (ProperStrategy P0 (SortedStrategy n0 ind sub1)) by eauto with inv.
@@ -1259,7 +1266,7 @@ Proof.
   1-2: specialize (all_in_union_left_most' H0); simpl; intros.
   1-2: specialize (proper_ms_sub_from_subfunc H12 H14 H4) as [Psub' Hsub'].
   1-2: eapply H5.
-  5,10: econstructor; [apply H29|constructor].
+  5,10: econstructor; [apply H30|constructor].
   1-8: simpl; eauto.
   1,3: specialize (proper_ms_sub_from_subfunc H10 H11 H4) as [Psub'' Hsub''];
       econstructor; eapply hm_sub_hm; eauto.
@@ -1276,12 +1283,12 @@ Proof.
   all: invcd H6.
   all: invcd H5.
   1,5: invcd_eval_value;
-    eapply H1; [ | | | | econstructor; [apply H18|constructor]];
+    eapply H1; [ | | | | econstructor; [apply H19|constructor]];
     simpl; eauto with eval union.
 
   all: invcd H0;
     specialize (all_in_union_left_most' H12); simpl; intros;
-    rewrite H19 in H0; invcd H0;
+    rewrite H20 in H0; invcd H0;
     solve_aiu.
   }
 
@@ -1297,7 +1304,7 @@ Proof.
     
   (* ISEq *)
   1-2: assert (fi = fi0) by eauto with union; subst.
-  1-2: rewrite H4 in H28; invcd H28.
+  1-2: rewrite H4 in H29; invcd H29.
   1-2: constructor; eauto.
   1-2: assert (HieraricalMergingInv P0 (SortedStrategy n0 ind sub1) tt) by eauto with inv.
   1-2: assert (ProperStrategy P0 (SortedStrategy n0 ind sub1)) by eauto with inv.
@@ -1306,7 +1313,7 @@ Proof.
   1-2: specialize (all_in_union_left_most' H0); simpl; intros.
   1-2: specialize (proper_ms_sub_from_subfunc H12 H14 H4) as [Psub' Hsub'].
   1-2: eapply H5.
-  5,10: econstructor; [apply H29|constructor].
+  5,10: econstructor; [apply H30|constructor].
   1-8: simpl; eauto.
   1,3: specialize (proper_ms_sub_from_subfunc H9 H10 H4) as [Psub'' Hsub''];
       econstructor; eapply hm_sub_hm; eauto.
@@ -1321,11 +1328,11 @@ Proof.
   all: invcd H6.
   all: invcd H5.
   1,6: invcd_eval_value;
-    eapply H1; [ | | | | econstructor; [apply H18|constructor]];
+    eapply H1; [ | | | | econstructor; [apply H19|constructor]];
     simpl; eauto with eval union.
 
   all: invcd H0; specialize (all_in_union_left_most' H12); simpl; intros.
-  1,5: rewrite H19 in H0; invcd H0;
+  1,5: rewrite H20 in H0; invcd H0;
     solve_aiu.
   all: rewrite H17 in H0; invcd H0;
     solve_aiu.
@@ -1337,14 +1344,14 @@ Proof.
   all: invcd H9.
   all: invcd H8.
   2,7: invcd_eval_value;
-    eapply H4; [ | | | | econstructor; [apply H26|constructor]];
+    eapply H4; [ | | | | econstructor; [apply H27|constructor]];
     simpl; eauto with eval union.
 
-  1,5: invcd H20; specialize (all_in_union_left_most' H15); simpl; intros;
+  1,5: invcd H21; specialize (all_in_union_left_most' H15); simpl; intros;
   rewrite H8 in H1; invcd H1; solve_aiu.
 
   all: invcd H2; specialize (all_in_union_left_most' H15); simpl; intros;
-  rewrite H25 in H2; invcd H2; solve_aiu.
+  rewrite H26 in H2; invcd H2; solve_aiu.
   }
 
   (* II* *)
@@ -1367,27 +1374,27 @@ Proof.
   econstructor; eauto with inv eval.
 
   1-2: assert (fti = fti0) by eauto with union; subst.
-  1-2: rewrite H6 in H35; invcd H35.
+  1-2: rewrite H6 in H36; invcd H36.
   1-2: assert (HieraricalMergingInv P0 (SortedStrategy n0 ind sub1) tt) by eauto with inv.
   1-2: assert (HieraricalMergingInv P0 (SortedStrategy n0 ind sub1) ft) by eauto with inv.
   1-2: assert (ProperStrategy P0 (SortedStrategy n0 ind sub1)) by eauto with inv.
   1-2: assert (ProperStrategy Psub (SortedStrategy n0 ind sub1)) by eauto with sub.
-  1-2: specialize (all_in_union_left_most' H29); simpl; intro.
-  1-2: specialize (all_in_union_left_most' H31); simpl; intros.
+  1-2: specialize (all_in_union_left_most' H30); simpl; intro.
+  1-2: specialize (all_in_union_left_most' H32); simpl; intros.
   1-2: specialize (proper_ms_sub_from_subfunc H14 H17 H6) as [Psub' Hsub'].
   1-2: eapply H7.
-  5,10: econstructor; [apply H36|constructor].
+  5,10: econstructor; [apply H37|constructor].
   1-8: simpl; eauto.
   1,3: specialize (proper_ms_sub_from_subfunc H13 H17 H6) as [Psub'' Hsub''];
       econstructor; eapply hm_sub_hm; eauto.
   1,2: eapply sub_subrt_subrt; eauto.
 Qed.
 
-Theorem eval_do_not_change_index_subrt_eq' : forall {T n n1} {P ind sub} {i t} {Psub} {s : MergingStrategy T n1},
+Theorem eval_do_not_change_index_subrt_eq' : forall {T n n1} {P ind sub} {i t} {Psub} {s : MergingStrategy T n1} {step},
   SubStrategyRT Psub P s (SortedStrategy n ind sub) ->
   EvalTermsGood s t ->
   all_in_et (fun (x : T) => ind x = Some i) t ->
-  forall u, t ==>* (EvalValue s u) ->
+  forall u, t ==>(step)* (EvalValue s u) ->
   AllInUnion (fun (x : T) => ind x = Some i) u.
 Proof.
   intros.
@@ -1395,11 +1402,11 @@ Proof.
   eapply (eval_do_not_change_index_subrt true); eauto.
 Qed.
 
-Theorem eval_do_not_change_index_subrt_lowerbound' : forall {T n n1} {P ind sub} {i t} {Psub} {s : MergingStrategy T n1},
+Theorem eval_do_not_change_index_subrt_lowerbound' : forall {T n n1} {P ind sub} {i t} {Psub} {s : MergingStrategy T n1} {step},
   SubStrategyRT Psub P s (SortedStrategy n ind sub) ->
   EvalTermsGood s t ->
   all_in_et (fun x => exists i1, ind x = Some i1 /\ (i1 > i)%Z) t ->
-  forall u, t ==>* (EvalValue s u) ->
+  forall u, t ==>(step)* (EvalValue s u) ->
   AllInUnion (fun x => exists i1, ind x = Some i1 /\ (i1 > i)%Z) u.
 Proof.
   intros.
@@ -1407,10 +1414,10 @@ Proof.
   eapply (eval_do_not_change_index_subrt false); eauto.
 Qed.
 
-Theorem eval_do_not_change_index_eq' : forall {T n} {ind sub} {i t},
+Theorem eval_do_not_change_index_eq' : forall {T n} {ind sub} {i t} {step},
   EvalTermsGood (SortedStrategy n ind sub) t ->
   all_in_et (fun (x : T) => ind x = Some i) t ->
-  forall u, t ==>* (EvalValue (SortedStrategy n ind sub) u) ->
+  forall u, t ==>(step)* (EvalValue (SortedStrategy n ind sub) u) ->
   AllInUnion (fun (x : T) => ind x = Some i) u.
 Proof.
   intros.
@@ -1420,11 +1427,11 @@ Qed.
 
 #[global] Hint Resolve eval_do_not_change_index_eq' : eval.
 
-Theorem eval_do_not_change_index_sub_eq' : forall {T n n1} {P ind sub} {i t} {Psub} {s : MergingStrategy T n1},
+Theorem eval_do_not_change_index_sub_eq' : forall {T n n1} {P ind sub} {i t} {Psub} {s : MergingStrategy T n1} {step},
   SubStrategy Psub P i s (SortedStrategy n ind sub) ->
   EvalTermsGood s t ->
   all_in_et (fun (x : T) => ind x = Some i) t ->
-  forall u, t ==>* (EvalValue s u) ->
+  forall u, t ==>(step)* (EvalValue s u) ->
   AllInUnion (fun (x : T) => ind x = Some i) u.
 Proof.
   intros.
@@ -1433,10 +1440,10 @@ Qed.
 
 #[global] Hint Resolve eval_do_not_change_index_sub_eq' : eval.
 
-Theorem eval_do_not_change_index_lowerbound' : forall {T n} {ind sub} {i t},
+Theorem eval_do_not_change_index_lowerbound' : forall {T n} {ind sub} {i t} {step},
   EvalTermsGood (SortedStrategy n ind sub) t ->
   all_in_et (fun x => exists i1, ind x = Some i1 /\ (i1 > i)%Z) t ->
-  forall u, (t : EvalTerms T) ==>* (EvalValue (SortedStrategy n ind sub) u) ->
+  forall u, (t : EvalTerms T) ==>(step)* (EvalValue (SortedStrategy n ind sub) u) ->
   AllInUnion (fun x => exists i1, ind x = Some i1 /\ (i1 > i)%Z) u.
 Proof.
   intros.
@@ -1446,12 +1453,12 @@ Qed.
 
 #[global] Hint Resolve eval_do_not_change_index_lowerbound' : eval.
 
-Theorem eval_do_not_change_index_sub_lowerbound' : forall {T n n1} {P ind sub} {i t} {Psub} {s : MergingStrategy T n1},
+Theorem eval_do_not_change_index_sub_lowerbound' : forall {T n n1} {P ind sub} {i t} {Psub} {s : MergingStrategy T n1} {step},
   ProperStrategy P (SortedStrategy n ind sub) ->
   SubStrategy Psub P i s (SortedStrategy n ind sub) ->
   EvalTermsGood s t ->
   all_in_et (fun x => exists i1, ind x = Some i1 /\ (i1 > i)%Z) t ->
-  forall u, t ==>* (EvalValue s u) ->
+  forall u, t ==>(step)* (EvalValue s u) ->
   AllInUnion (fun x => exists i1, ind x = Some i1 /\ (i1 > i)%Z) u.
 Proof.
   intros.
@@ -1461,11 +1468,11 @@ Qed.
 #[global] Hint Resolve eval_do_not_change_index_sub_lowerbound' : eval.
 
 
-Theorem eval_do_not_change_index_subrt_eq : forall {T n n1} {P ind sub} {i t} {Psub} {s : MergingStrategy T n1},
+Theorem eval_do_not_change_index_subrt_eq : forall {T n n1} {P ind sub} {i t} {Psub} {s : MergingStrategy T n1} {step},
   SubStrategyRT Psub P s (SortedStrategy n ind sub) ->
   EvalTermsGood s t ->
   all_in_et (fun (x : T) => ind x = Some i) t ->
-  forall u, t ==> (EvalValue s u) ->
+  forall u, t ==>(step) (EvalValue s u) ->
   AllInUnion (fun (x : T) => ind x = Some i) u.
 Proof.
   intros.
@@ -1473,11 +1480,11 @@ Proof.
   eapply (eval_do_not_change_index_subrt true); eauto with eval.
 Qed.
 
-Theorem eval_do_not_change_index_subrt_lowerbound : forall {T n n1} {P ind sub} {i t} {Psub} {s : MergingStrategy T n1},
+Theorem eval_do_not_change_index_subrt_lowerbound : forall {T n n1} {P ind sub} {i t} {Psub} {s : MergingStrategy T n1} {step},
   SubStrategyRT Psub P s (SortedStrategy n ind sub) ->
   EvalTermsGood s t ->
   all_in_et (fun x => exists i1, ind x = Some i1 /\ (i1 > i)%Z) t ->
-  forall u, t ==> (EvalValue s u) ->
+  forall u, t ==>(step) (EvalValue s u) ->
   AllInUnion (fun x => exists i1, ind x = Some i1 /\ (i1 > i)%Z) u.
 Proof.
   intros.
@@ -1485,10 +1492,10 @@ Proof.
   eapply (eval_do_not_change_index_subrt false); eauto with eval.
 Qed.
 
-Theorem eval_do_not_change_index_eq : forall {T n} {ind sub} {i t},
+Theorem eval_do_not_change_index_eq : forall {T n} {ind sub} {i t} {step},
   EvalTermsGood (SortedStrategy n ind sub) t ->
   all_in_et (fun (x : T) => ind x = Some i) t ->
-  forall u, t ==> (EvalValue (SortedStrategy n ind sub) u) ->
+  forall u, t ==>(step) (EvalValue (SortedStrategy n ind sub) u) ->
   AllInUnion (fun (x : T) => ind x = Some i) u.
 Proof.
   intros.
@@ -1498,11 +1505,11 @@ Qed.
 
 #[global] Hint Resolve eval_do_not_change_index_eq : eval.
 
-Theorem eval_do_not_change_index_sub_eq : forall {T n n1} {P ind sub} {i t} {Psub} {s : MergingStrategy T n1},
+Theorem eval_do_not_change_index_sub_eq : forall {T n n1} {P ind sub} {i t} {Psub} {s : MergingStrategy T n1} {step},
   SubStrategy Psub P i s (SortedStrategy n ind sub) ->
   EvalTermsGood s t ->
   all_in_et (fun (x : T) => ind x = Some i) t ->
-  forall u, t ==> (EvalValue s u) ->
+  forall u, t ==>(step) (EvalValue s u) ->
   AllInUnion (fun (x : T) => ind x = Some i) u.
 Proof.
   intros.
@@ -1511,10 +1518,10 @@ Qed.
 
 #[global] Hint Resolve eval_do_not_change_index_sub_eq : eval.
 
-Theorem eval_do_not_change_index_lowerbound : forall {T n} {ind sub} {i t},
+Theorem eval_do_not_change_index_lowerbound : forall {T n} {ind sub} {i t} {step},
   EvalTermsGood (SortedStrategy n ind sub) t ->
   all_in_et (fun x => exists i1, ind x = Some i1 /\ (i1 > i)%Z) t ->
-  forall u, (t : EvalTerms T) ==> (EvalValue (SortedStrategy n ind sub) u) ->
+  forall u, (t : EvalTerms T) ==>(step) (EvalValue (SortedStrategy n ind sub) u) ->
   AllInUnion (fun x => exists i1, ind x = Some i1 /\ (i1 > i)%Z) u.
 Proof.
   intros.
@@ -1524,12 +1531,12 @@ Qed.
 
 #[global] Hint Resolve eval_do_not_change_index_lowerbound : eval.
 
-Theorem eval_do_not_change_index_sub_lowerbound : forall {T n n1} {P ind sub} {i t} {Psub} {s : MergingStrategy T n1},
+Theorem eval_do_not_change_index_sub_lowerbound : forall {T n n1} {P ind sub} {i t} {Psub} {s : MergingStrategy T n1} {step},
   ProperStrategy P (SortedStrategy n ind sub) ->
   SubStrategy Psub P i s (SortedStrategy n ind sub) ->
   EvalTermsGood s t ->
   all_in_et (fun x => exists i1, ind x = Some i1 /\ (i1 > i)%Z) t ->
-  forall u, t ==> (EvalValue s u) ->
+  forall u, t ==>(step) (EvalValue s u) ->
   AllInUnion (fun x => exists i1, ind x = Some i1 /\ (i1 > i)%Z) u.
 Proof.
   intros.
@@ -1537,24 +1544,4 @@ Proof.
 Qed.
 
 #[global] Hint Resolve eval_do_not_change_index_sub_lowerbound : eval.
-
-  (*
-Lemma eval_reduce_metric : forall {T n} {t t1 : EvalTerms T} {ms : MergingStrategy T n},
-  EvalTermsGood ms t ->
-  t ==> t1 ->
-  metric t1 < metric t.
-Proof.
-  intros.
-  destruct t.
-  - inversion H0.
-  - invcd H0; simpl; try lia.
-  - invcd H0; simpl; try lia.
-    unfold ms_depth. lia.
-  - admit.
-  - admit.
-  - admit.
-Admitted.
-
-#[global] Hint Resolve eval_reduce_metric : eval.
-*)
 
